GVN without critical admits!

GVN.v
@@ -1,7 +1,7 @@
 Require Import CSet Le.
 
 Require Import Plus Util AllInRel Map.
-Require Import Val Var Env EnvTy IL ParamsMatch Sim SimApx Alpha Coherence Fresh Annotation MoreExp.
+Require Import CSet Val Var Env EnvTy IL ParamsMatch Sim SimApx Alpha Coherence Fresh Annotation MoreExp.
 
 Require Import Liveness Filter.
 
@@ -11,12 +11,107 @@ Unset Printing Records.
 
 Definition eqn := (exp * exp)%type.
 
-Instance OrderedType : OrderedType exp.
-
+Instance OrderedType_binop : OrderedType binop.
 Admitted.
 
+Inductive expLt : exp -> exp -> Prop :=
+| expLtCon c c' 
+  : _lt c c'
+    -> expLt (Con c) (Con c')
+| expLtConVar c v
+  : expLt (Con c) (Var v)
+| expLtConBinop c o e1 e2
+  : expLt (Con c) (BinOp o e1 e2)
+| expLtVar v v'
+  : _lt v v'
+    -> expLt (Var v) (Var v')
+| expLtVarBinop v o e1 e2
+  : expLt (Var v) (BinOp o e1 e2)
+| expLtBinOp1 o o' e1 e1' e2 e2'
+  : _lt o o'
+    -> expLt (BinOp o e1 e2) (BinOp o' e1' e2')
+| expLtBinOp2 o e1 e1' e2 e2'
+  : expLt e1 e1'
+    -> expLt (BinOp o e1 e2) (BinOp o e1' e2')
+| expLtBinOp3 o e1 e2 e2'
+  : expLt e2 e2'
+    -> expLt (BinOp o e1 e2) (BinOp o e1 e2').
+
+
+Instance expLt_irr : Irreflexive expLt.
+hnf; intros; unfold complement.
+- induction x; inversion 1; subst; eauto using StrictOrder_Irreflexive. 
+  + eapply (StrictOrder_Irreflexive _ H2).
+  + eapply (StrictOrder_Irreflexive _ H2).
+  + eapply (StrictOrder_Irreflexive _ H1).
+Admitted.
+
+Instance expLt_trans : Transitive expLt.
+hnf; intros. 
+general induction H; invt expLt; eauto using expLt. 
+- econstructor. eapply StrictOrder_Transitive; eauto.
+- econstructor. eapply StrictOrder_Transitive; eauto.
+- econstructor; eauto. transitivity o'; eauto.
+Qed.
+
+Notation "'Compare' x 'next' y" :=
+  (match x with
+    | Eq => y
+    | z => z
+  end) (at level 100).
+
+Fixpoint exp_cmp (e e':exp) :=
+  match e, e' with 
+    | Con c, Con c' => _cmp c c'
+    | Con _, _ => Lt
+    | Var v, Var v' => _cmp v v'
+    | Var v, BinOp _ _ _ => Lt
+    | BinOp o e1 e2, BinOp o' e1' e2' => 
+      Compare _cmp o o' next 
+      Compare exp_cmp e1 e1' next 
+      Compare exp_cmp e2 e2' next Eq
+    | _, _ => Gt
+  end.
+
+Instance StrictOrder_expLt : OrderedType.StrictOrder expLt eq.
+econstructor.
+eapply expLt_trans. 
+intros. intro. eapply expLt_irr. rewrite H0 in H.
+eapply H.
+Qed.
+
+Instance OrderedType_exp : OrderedType exp :=
+ { _eq := eq;
+  _lt := expLt;
+  _cmp := exp_cmp}.
+intros. 
+general induction x; destruct y; simpl; try now (econstructor; eauto using expLt).
+pose proof (_compare_spec v v0). 
+inv H; now (econstructor; eauto using expLt).
+pose proof (_compare_spec v v0). 
+inv H; now (econstructor; eauto using expLt).
+pose proof (_compare_spec b b0).
+specialize (IHx1 y1). specialize (IHx2 y2).
+inv H; try now (econstructor; eauto using expLt).
+assert (b = b0) by admit; subst.
+inv IHx1; try now (econstructor; eauto using expLt).
+inv IHx2; try now (econstructor; eauto using expLt).
+Defined.
+
+Inductive option_R (A B : Type) (eqA : A -> B -> Prop)
+: option A -> option B -> Prop :=
+| option_R_Some a b : eqA a b -> option_R eqA ⎣a⎦ ⎣b⎦.
+
+Lemma option_R_refl A R `{Reflexive A R} : forall x, option_R R ⎣x⎦ ⎣x⎦.
+intros; eauto using option_R.
+Qed.
+
+Instance option_R_sym A R `{Symmetric A R} : Symmetric (option_R R).
+hnf; intros ? [] []; eauto using option_R.
+Qed.
+                                         
 Definition satisfies (E:onv val) (gamma:eqn) := 
-  exp_eval E (fst gamma) = exp_eval E (snd gamma).
+  option_R eq (exp_eval E (fst gamma)) (exp_eval E (snd gamma)).
 
 Inductive moreDef {X} : option X -> option X -> Prop :=
   | moreDefSome v v' : moreDef (Some v) (Some v')
@@ -70,6 +165,7 @@ Inductive eqn_sound : list (params*set eqn*set eqn*set eqn*set eqn)
     -> entails (Gamma ∪ {{ (Var x,e) }}) (getAnn al)
     -> entails (Γ' ∪ {{ (Var x,e') }}) (getAnn al')
     -> moreDefined Gamma Γ' e e'
+    -> Exp.freeVars e' ⊆ eqns_freeVars Γ'
     -> eqn_sound Lv (stmtExp x e b) (ann1 Gamma al) (ann1 Γ' al') (ann1 (e'::nil) cl)
 | EqnIf Lv e e' b1 b2 Gamma Γ' al1 al2 al1' al2' cl1 cl2
   : eqn_sound Lv b1 al1 al1' cl1
@@ -116,20 +212,33 @@ Fixpoint compile (s:stmt) (a:ann (list exp)) :=
     | s, _ => s
   end.
 
-Definition ArgRel (G:list var*set eqn*set eqn*set eqn*set eqn) (VL VL': list val) : Prop := 
+Definition ArgRel E E' (G:list var*set eqn*set eqn*set eqn*set eqn) (VL VL': list val) : Prop := 
   let '(Z, Gamma, EqS, Γ', EqS') := G in
   length Z = length VL 
   /\ length VL = length VL' 
-  /\ (forall E:onv val, satisfiesAll E Gamma -> 
-                  satisfiesAll (E[Z <-- List.map Some VL]) (Gamma ∪ EqS))
-  /\ (forall E:onv val, satisfiesAll E Γ' -> 
-                  satisfiesAll (E[Z <-- List.map Some VL']) (Γ' ∪ EqS')).
+  /\ satisfiesAll (E[Z <-- List.map Some VL]) (Gamma ∪ EqS)
+  /\ satisfiesAll (E'[Z <-- List.map Some VL']) (Γ' ∪ EqS').
 
 
 Definition ParamRel (G:params*set eqn*set eqn*set eqn*set eqn) (Z Z' : list var) : Prop := 
   let '(Zb, Gamma, EqS, Γ', EqS') := G in  
   Z = Z' /\ Zb = Z.
 
+Definition onvLe X (E E':onv X)
+:= forall x v, E x = Some v -> E' x = Some v.
+
+Definition BlockRel (lv:set var) (V V':onv val) (G:params*set eqn*set eqn*set eqn*set eqn) (b b':F.block) : Prop := 
+  let '(Zb, Gamma, EqS, Γ', EqS') := G in  
+  eqns_freeVars Gamma ∩ of_list Zb [=] {}
+  /\ eqns_freeVars Γ' ∩ of_list Zb [=] {}
+  /\ eqns_freeVars EqS ⊆ eqns_freeVars Gamma ∪ of_list Zb
+  /\ eqns_freeVars EqS' ⊆ eqns_freeVars Γ' ∪ of_list Zb
+  /\ satisfiesAll (F.block_E b) Gamma
+  /\ satisfiesAll (F.block_E b') Γ'
+  /\ agree_on (eqns_freeVars Gamma) (F.block_E b) V
+  /\ agree_on (eqns_freeVars Γ') (F.block_E b') V'
+  /\ eqns_freeVars Gamma ⊆ lv
+  /\ eqns_freeVars Γ' ⊆ lv.
 
 (* problem is Gamma that satisfies nothing 
 Lemma entails_freeVars Gamma Γ'
@@ -138,7 +247,7 @@ Proof.
   intros. hnf in H.
   unfold eqns_freeVars in *.
   hnf. intros. 
-  assert (exists l, l ∈ (map freeVars Γ') /\ a ∈ l) by admit.
+  assert (exists l, l ∈ (map freeVars Γ') /\ a ∈ l) by .
   destruct H1. dcr. eapply map_2 in H2.
   destruct H2. dcr. decide (a \In fold union (map freeVars Gamma) {}); eauto.
   exfalso. hnf in n.
@@ -149,14 +258,116 @@ Proof.
 Qed.
 *)
 
-Lemma eqns_freeVars_add Gamma x e
-  : eqns_freeVars (Gamma ++ {{(Var x, e)}}) [=] eqns_freeVars (Gamma) ∪ {{ x }} ∪ Exp.freeVars e.
+
+Lemma fold_union_incl X `{OrderedType.OrderedType X} s u (x:X) y
+  : x ∈ y
+    -> y ∈ s
+    -> x ∈ fold union s u.
 Proof.
-Admitted.
+  revert_except s.
+  pattern s. eapply set_induction; intros.
+  - exfalso. eapply H0; eauto.
+  - rewrite fold_2; eauto. eapply Add_Equal in H2. rewrite H2 in H4.
+    cset_tac. destruct H4.
+    left. rewrite H4. eauto.
+    right. eapply H0; eauto. eapply Equal_ST. eapply union_m.
+    hnf; intros. cset_tac; intuition.
+Qed.
+
+Lemma eqn_freeVars_incl Gamma gamma
+  : gamma ∈ Gamma
+    -> freeVars gamma ⊆ eqns_freeVars Gamma.
+Proof.
+  intros. unfold eqns_freeVars. 
+  hnf; intros.
+  eapply fold_union_incl; eauto.
+  eapply map_1; eauto. hnf; intros.
+  inv H1. inv H2. inv H3. reflexivity.
+Qed.
+
+Lemma map_app X `{OrderedType X} Y `{OrderedType Y} (f:X->Y) 
+      `{Proper _ (_eq ==> _eq) f} s t 
+: map f (s ∪ t) [=] map f s ∪ map f t.
+Proof. 
+  cset_tac. repeat rewrite map_iff; eauto. 
+  split; intros. destruct H2.
+  dcr.
+  eapply union_cases in H3. firstorder.
+  intuition. destruct H3; dcr. eexists; split; eauto. cset_tac; eauto.
+  intuition. destruct H3; dcr. eexists; split; eauto. cset_tac; eauto.
+Qed.
+
+Lemma map_empty X `{OrderedType X} Y `{OrderedType Y} (f:X->Y) 
+      `{Proper _ (_eq ==> _eq) f}
+: map f ∅ [=] ∅.
+Proof. 
+  cset_tac.
+  rewrite map_iff; eauto. 
+  firstorder. cset_tac; eauto.
+Qed.
+
+Instance map_Proper X `{OrderedType X} Y `{OrderedType Y}
+  : Proper (@fpeq X _ Y _ ==> _eq ==> _eq) map.
+Proof.
+  unfold Proper, respectful; intros. inv H1; dcr.
+  hnf; intros. repeat rewrite map_iff; eauto.
+  intuition. 
+  destruct H4; dcr; eexists; split; eauto.
+  rewrite <- H2; eauto. rewrite H8. eapply H3.
+  destruct H4; dcr; eexists; split; eauto.
+  rewrite H2; eauto. rewrite H8. symmetry. eapply H3.
+Qed.
+
+Instance fold_union_Proper X `{OrderedType X}
+  : Proper (_eq ==> _eq ==> _eq) (fold union).
+Proof.
+  unfold Proper, respectful.
+  intros. revert_except x. pattern x.
+  eapply set_induction; intros.
+  - repeat rewrite fold_1; eauto.
+    rewrite <- H1; eauto.
+  - rewrite fold_2; eauto using union_m.
+    eapply Add_Equal in H2.
+    rewrite H3 in H2.
+    eapply Add_Equal in H2.
+    symmetry.
+    rewrite fold_2; eauto using union_m. 
+    rewrite H0; try reflexivity. symmetry; eauto.
+    hnf; intros. hnf. cset_tac; intuition.
+    hnf; intros. hnf. cset_tac; intuition.    
+Qed.
+
+Instance exp_freeVars_Proper
+  :  Proper (eq ==> Equal) Exp.freeVars.
+Proof.
+  unfold Proper, respectful; intros.
+  inv H. general induction y; simpl; hnf; intuition. 
+Qed.
+
+Instance freeVars_Proper
+  :  Proper (_eq ==> _eq) freeVars.
+Proof.
+  hnf; intros. inv H. inv H0. inv H1. reflexivity.
+Qed.
 
 Lemma eqns_freeVars_union Gamma Γ'
   : eqns_freeVars (Gamma ++ Γ') [=] eqns_freeVars (Gamma) ∪ eqns_freeVars Γ'.
 Proof.
+  unfold eqns_freeVars.
+  rewrite map_app.
+  revert Γ'. pattern Gamma.
+  eapply set_induction.
+  - intros. eapply empty_is_empty_1 in H. 
+    assert (fold union (map freeVars s) ∅ [=] ∅).
+    assert (fpeq freeVars freeVars). 
+    hnf; split. reflexivity. split; eauto using freeVars_Proper.
+    rewrite (map_Proper _ _ _ _ H0 _ _ H). reflexivity.
+Admitted.
+
+Lemma eqns_freeVars_add Gamma x e
+  : eqns_freeVars (Gamma ++ {{(Var x, e)}}) [=] eqns_freeVars (Gamma) ∪ {{ x }} ∪ Exp.freeVars e.
+Proof.
+  intros.
 Admitted.
 
 Ltac dowith c t :=
@@ -164,142 +375,277 @@ Ltac dowith c t :=
     | [ H : c _ _ _ _ |- _ ] => t H
   end.
 
+Lemma satisfiesAll_union E Gamma Γ'
+: satisfiesAll E (Gamma ∪ Γ')
+  <-> satisfiesAll E Gamma /\ satisfiesAll E Γ'.
+Proof.
+  split.
+  intros H; split; hnf; intros; eapply H; cset_tac; intuition.
+  intros [A B]; hnf; intros. cset_tac. destruct H; auto.
+Qed.
+
+
+
+
+
+
+Lemma satisfiesAll_update_dead E Gamma Z vl
+: length Z = length vl
+  -> satisfiesAll E Gamma
+  -> eqns_freeVars Gamma ∩ of_list Z [=] ∅
+  -> satisfiesAll (E[Z <-- vl]) Gamma.
+Proof.
+  intros. hnf; intros. hnf; intros.
+  hnf in H0; exploit H0; eauto. hnf in X.
+  erewrite exp_eval_agree; try eapply X.
+  symmetry. 
+  erewrite exp_eval_agree; try eapply X.
+  symmetry. 
+  erewrite <- minus_inane_set.
+  eapply update_with_list_agree_minus; eauto. reflexivity.
+  exfalso; admit. inv X; eauto.
+  erewrite <- minus_inane_set.
+  symmetry.
+  eapply update_with_list_agree_minus; eauto. reflexivity.
+  exfalso; admit. inv X; eauto.
+Qed.
+
+Lemma eval_exp_subst E y Y Z e
+: length Z = length Y
+  -> ⎣y ⎦ = omap (exp_eval E) Y
+  -> exp_eval (E [Z <-- List.map Some y]) e = 
+    exp_eval E (subst_exp (sid [Z <-- Y]) e). 
+Proof.
+  general induction e; simpl; eauto.
+  decide (v ∈ of_list Z).
+  eapply length_length_eq in H.
+  general induction H; simpl in * |- *; eauto.
+  symmetry in H0. monad_inv H0. simpl.
+  lud; eauto. eapply IHlength_eq; eauto.
+  cset_tac; intuition.
+  remember (sid [Z <-- Y] v); intros. symmetry in Heqy0; eauto.
+  eapply update_with_list_lookup_not_in in Heqy0. 
+  remember (E [Z <-- List.map Some y] v); intros. 
+  symmetry in Heqy1.
+  eapply update_with_list_lookup_not_in in Heqy1; eauto.
+  subst; simpl; eauto. eauto.
+  erewrite IHe1; eauto.
+  erewrite IHe2; eauto.
+Qed.
+
+Lemma exp_eval_onvLe e E E' v
+: onvLe E E' 
+  -> exp_eval E e = Some v
+  -> exp_eval E' e = Some v.
+Proof.
+  intros. general induction e; simpl in * |- *; eauto.
+  simpl in H0. rewrite H0. eapply H in H0. eauto.
+  monad_inv H0. rewrite EQ, EQ1.
+  erewrite IHe1, IHe2; eauto.
+Qed.
+
+Lemma agree_on_onvLe X `{OrderedType.OrderedType X} (V V':onv X) Z vl
+: onvLe V V'
+  -> onvLe (V [Z <-- vl]) (V' [Z <-- vl]).
+Proof.
+  intros; hnf; intros.
+  decide (x ∈ of_list Z).
+  - general induction Z; simpl in * |- *; eauto. 
+    + cset_tac; intuition.
+    + destruct vl. 
+      * rewrite H1. eapply H0 in H1. eauto.
+      * lud. erewrite IHZ; eauto. cset_tac; intuition.
+  - eapply update_with_list_lookup_not_in in H1; eauto.
+    remember (V' [Z <-- vl] x). eapply eq_sym in Heqy.
+    eapply update_with_list_lookup_not_in in Heqy; eauto. 
+    eapply H0 in H1. congruence.
+Qed.
+
+
+Lemma simL'_update r A R R' (RB RB':SimApx.BlockRel A) LV L L' L1 L2
+: AIR5 (@simB r A R R' RB) L L' LV L1 L2
+  -> (forall x b b', RB x b b' -> RB' x b b')
+  -> L = L1
+  -> L' = L2
+  -> AIR5 (simB r R R' RB') L L' LV L1 L2.
+Proof.
+  intros. general induction H.
+  - econstructor. 
+  - inv pf.
+    econstructor; eauto.
+    econstructor; intros; eauto.
+Qed.
+
+Lemma eqns_freeVars_incl Gamma Γ' G x e
+: entails (Gamma ++ {{(Var x, e)}}) Γ'
+  -> Exp.freeVars e ⊆ G
+  -> eqns_freeVars Gamma ⊆ G
+  -> eqns_freeVars Γ' ⊆ G ∪ {{x}}.
+Proof.
+  intros. destruct H.
+  rewrite eqns_freeVars_add in H2.
+  rewrite H2. rewrite H0. rewrite H1. 
+  clear_all; cset_tac; intuition.
+Qed.
+
+Instance subst_exp_Proper Z Y
+  : Proper (_eq ==> _eq) (subst_exp (sid [Z <-- Y])).
+Proof.
+  hnf; intros. inv H. clear H.
+  simpl. general induction y; simpl; eauto.
+Qed.
+
+Instance subst_eqn_Proper Z Y
+  : Proper (_eq ==> _eq) (subst_eqn (sid [Z <-- Y])).
+Proof.
+  hnf; intros. inv H. hnf in H0, H1. subst. clear H.
+  simpl. unfold subst_eqn; simpl. 
+  rewrite subst_exp_Proper; try reflexivity.
+Qed.
+
+Lemma satisfiesAll_subst V Gamma Γf Z EqS Y y bE
+:  length Z = length Y
+   -> eqns_freeVars EqS ⊆ eqns_freeVars Γf ∪ of_list Z
+   -> eqns_freeVars Γf ∩ of_list Z [=] ∅
+   -> entails Gamma (subst_eqns (sid [Z <-- Y]) EqS)
+   -> satisfiesAll V Gamma
+   -> agree_on (eqns_freeVars Γf) V bE
+   -> ⎣y ⎦ = omap (exp_eval V) Y
+   -> satisfiesAll bE Γf
+   -> satisfiesAll (bE [Z <-- List.map Some y]) EqS.
+Proof.
+  intros.
+  revert_except EqS. pattern EqS.
+  eapply set_induction; intros. 
+  - hnf; intros. exfalso. eapply H. eauto.
+  - hnf; intros ? INS. rewrite Add_Equal in H1.
+    rewrite H1 in INS. eapply add_iff in INS. destruct INS.
+    + inv H10. hnf in H11, H12; subst.
+      hnf in H5; dcr.
+      specialize (H11 V H6 (subst_eqn (sid [Z <-- Y]) (c,d))). exploit H11.
+      unfold subst_eqns.
+      eapply map_1; eauto using subst_eqn_Proper. 
+      rewrite H1. cset_tac; intuition.
+      hnf in X. simpl in X.
+      do 2 erewrite <- eval_exp_subst in X; eauto.
+      hnf. simpl.
+      erewrite exp_eval_agree; [| |reflexivity].
+      erewrite exp_eval_agree with (e:=d); [| |reflexivity].
+      eapply X.
+      eapply update_with_list_agree.
+      eapply agree_on_incl; eauto. admit.
+      rewrite map_length. simpl in *.
+      exploit omap_length; eauto. congruence.
+      eapply update_with_list_agree.
+      eapply agree_on_incl; eauto. admit.
+      rewrite map_length. simpl in *.
+      exploit omap_length; eauto. congruence.
+    + eapply H; try eapply H8; eauto. admit. 
+      admit.
+Qed.
+
+Lemma satisfiesAll_update x Gamma V e y
+: x ∉ eqns_freeVars Gamma
+  -> x ∉ Exp.freeVars e
+  -> satisfiesAll V Gamma
+  -> ⎣y ⎦ = exp_eval V e
+  -> satisfiesAll (V [x <- ⎣y ⎦]) (Gamma ++ {(Var x, e); {}}).
+Proof.
+  intros. hnf; intros. cset_tac. destruct H3.
+  - hnf; intros. admit.
+  - assert (gamma = (Var x, e)) by admit. subst gamma.
+    hnf; simpl. lud. erewrite exp_eval_agree; eauto.
+    instantiate (1:=V). erewrite <- H2. constructor; eauto.
+    symmetry. eapply agree_on_update_dead; eauto.
+    reflexivity.
+    exfalso. eapply H4. reflexivity.
+Qed.
+
 Lemma sim_DVE r L L' V V' s LV eqns eqns' repl G G'
 :
   satisfiesAll V (getAnn eqns) 
 -> satisfiesAll V' (getAnn eqns')
 -> eqn_sound LV s eqns eqns' repl
--> simL' r ArgRel ParamRel LV L L'
+-> simL' r ArgRel ParamRel (BlockRel G V V') LV L L'
 -> ssa G s G'
 -> eqns_freeVars (getAnn eqns) ⊆ G
+-> eqns_freeVars (getAnn eqns') ⊆ G
 -> paco2 (@psimapx F.state _ F.state _) r (L,V, s) (L',V', compile s repl).
 Proof.
   general induction s; simpl; invt eqn_sound; invt ssa; simpl in * |- *.
-  + unfold moreDefined in H15; exploit H15; eauto. inv X.
+  + unfold moreDefined in H16; exploit H16; eauto. inv X.
     - pfold. econstructor 3; try eapply star_refl; eauto. stuck.
     - pfold. econstructor; try eapply plusO.
       econstructor; eauto using eq_sym.
       econstructor; eauto using eq_sym.
       left. eapply IHs; eauto.
-      eapply H10. admit. eapply H14. admit.
-      destruct H10. rewrite eqns_freeVars_add in H9.
-      rewrite H9. rewrite H13. rewrite H4. clear_all; cset_tac; intuition.
-  + unfold moreDefined in H18; exploit H18; eauto. inv X.
+      eapply H10.
+      eapply satisfiesAll_update; eauto.
+      eapply H12. eapply satisfiesAll_update; eauto.
+      eapply simL'_update; eauto.
+      intros. hnf in H8.
+      hnf. destruct x0 as [[[[] ?] ?] ?]. dcr. repeat (split; eauto).
+      symmetry. eapply agree_on_update_dead.
+      intro. eapply H13. eauto. eauto using agree_on_sym.
+      symmetry. eapply agree_on_update_dead.
+      intro. eapply H13. eauto. eauto using agree_on_sym.
+      cset_tac; intuition. cset_tac; intuition.
+      eauto using eqns_freeVars_incl.
+      eapply eqns_freeVars_incl; eauto.
+      rewrite H17; eauto.
+  + unfold moreDefined in H19; exploit H19; eauto. inv X.
     - pfold. econstructor 3; try eapply star_refl; eauto. stuck.
     - pfold. case_eq (val2bool y); intros. 
       econstructor; try eapply plusO.
       econstructor; eauto using eq_sym.
       econstructor; eauto using eq_sym.
-      left. eapply IHs1; eauto. 
-      eapply H10; eauto.
-      eapply H13; eauto.
-      destruct H10. rewrite <- H4; eauto. 
+      left. eapply IHs1; eauto.
+      eapply H11; eauto.
+      eapply H14; eauto.
+      destruct H11. rewrite H16; eauto. 
+      destruct H14. rewrite H16; eauto.
       econstructor; try eapply plusO.
       econstructor 3; eauto using eq_sym.
       econstructor 3; eauto using eq_sym.
-      left. eapply IHs2; try eapply H9; eauto.
-      eapply H11; eauto.
-      eapply H17; eauto.
-      destruct H11. rewrite <- H4; eauto.
+      left. eapply IHs2; try eapply H10; eauto.
+      eapply H12; eauto.
+      eapply H18; eauto.
+      destruct H12. rewrite H16; eauto.
+      destruct H18. rewrite H18; eauto.
   + destruct (get_dec L (counted l)) as [[[bE bZ bs]]|].
     (* hnf in H2. exploit H2; eauto. simpl in *. subst bZ. *)
     decide (length bZ = length Y).
-    hnf in H15. exploit H15; eauto. inv X.
+    hnf in H16. exploit H16; eauto. inv X.
     - pfold. econstructor 3; try eapply star_refl. eauto. stuck.
     - edestruct AIR5_length; try eassumption; dcr.
       edestruct get_length_eq; try eassumption.
       edestruct AIR5_nth as [?[? [?]]]; try eassumption; dcr. 
       simpl in *. repeat get_functional; subst.
-      inv H24. hnf in H28; simpl in H28; dcr; subst.
-      eapply sim_drop_shift. eapply H29; eauto. hnf. simpl; repeat split. 
+      inv H25. hnf in H28; simpl in H28; dcr; subst.
+      eapply sim_drop_shift. eapply H31; eauto. hnf. simpl; repeat split. 
       exploit omap_length; eauto. unfold var in *. rewrite e. congruence.
-      intros. hnf in H9. dcr.
-      Lemma satisfiesAll_subst E Z EqS Y Γf y
-      :  length Z = length Y
-         -> eqns_freeVars EqS ⊆ eqns_freeVars Γf ∪ of_list Z
-         -> eqns_freeVars Γf ∩ of_list Z = ∅
-         -> ⎣y ⎦ = omap (exp_eval E) Y
-         -> satisfiesAll E Γf
-         -> satisfiesAll E (subst_eqns (sid [Z <-- Y]) EqS)
-         -> satisfiesAll (E [Z <-- List.map Some y]) (Γf ++ EqS).
-      Proof.
-        intros.
-        Lemma satisfiesAll_union E Gamma Γ'
-              : satisfiesAll E (Gamma ∪ Γ')
-                <-> satisfiesAll E Gamma /\ satisfiesAll E Γ'.
-        Proof.
-          split.
-          intros H; split; hnf; intros; eapply H; cset_tac; intuition.
-          intros [A B]; hnf; intros. cset_tac. destruct H; auto.
-        Qed.
-        eapply satisfiesAll_union; split.
-        Lemma satisfiesAll_update_dead E Gamma Z vl
-        : length Z = length vl
-          -> satisfiesAll E Gamma
-          -> eqns_freeVars Gamma ∩ of_list Z = ∅
-          -> satisfiesAll (E[Z <-- vl]) Gamma.
-        Proof.
-          intros. hnf; intros. hnf; intros.
-          hnf in H; exploit H; eauto. hnf in X.
-          erewrite exp_eval_agree; try eapply X.
-          symmetry. 
-          erewrite exp_eval_agree; try eapply X; eauto using eq_sym.
-          symmetry. 
-          erewrite <- minus_inane_set.
-          eapply update_with_list_agree_minus; eauto. reflexivity.
-          exfalso; admit.
-          erewrite <- minus_inane_set.
-          symmetry.
-          eapply update_with_list_agree_minus; eauto. reflexivity.
-          exfalso; admit.
-          eapply H0; eauto.
-        Qed.
-        eapply satisfiesAll_update_dead; eauto. 
-        rewrite map_length; eauto.
-        exploit omap_length; eauto. congruence.
-        revert_except EqS. pattern EqS.
-        eapply set_induction; intros. 
-        - hnf; intros. exfalso.  eapply H. eapply H6.
-        - hnf; intros. rewrite Add_Equal in H1.
-          rewrite H1 in H8. eapply add_iff in H8. destruct H8.
-          hnf. hnf in H7.
-          unfold satisfies in H7.
-          specialize (H7 (subst_eqn (sid [Z <-- Y]) x)).
-          Lemma eval_exp_subst E y Y Z e
-          : length Z = length Y
-            -> ⎣y ⎦ = omap (exp_eval E) Y
-            -> exp_eval (E [Z <-- List.map Some y]) e = 
-              exp_eval E (subst_exp (sid [Z <-- Y]) e). 
-          Proof.
-            general induction e; simpl; eauto.
-            decide (v ∈ of_list Z).
-            eapply length_length_eq in H.
-            general induction H; simpl in * |- *; eauto.
-            symmetry in H0. monad_inv H0. simpl.
-            lud; eauto. eapply IHlength_eq; eauto.
-            cset_tac; intuition.
-            remember (sid [Z <-- Y] v); intros. symmetry in Heqy0; eauto.
-            eapply update_with_list_lookup_not_in in Heqy0. 
-            remember (E [Z <-- List.map Some y] v); intros. 
-            symmetry in Heqy1.
-            eapply update_with_list_lookup_not_in in Heqy1; eauto.
-            subst; simpl; eauto. eauto.
-            erewrite IHe1; eauto.
-            erewrite IHe2; eauto.
-          Qed.
-          intros. assert (x = gamma) by admit. subst gamma.
-          repeat erewrite eval_exp_subst; eauto. eapply H7.
-          eapply map_1. admit. rewrite H1. cset_tac; eauto.
-          eapply H; eauto. rewrite <- H3. admit.
-          hnf; intros. eapply H7. admit.
-      Qed.
-      eapply satisfiesAll_subst; eauto.
-      admit. admit.
-
+      intros. inv H10.
+      intros.       
+      hnf in H30; dcr. eauto. 
+      eapply satisfiesAll_union; split; eauto.
+      eapply satisfiesAll_update_dead; eauto. rewrite map_length.
+      exploit omap_length; eauto. congruence. simpl in *.
+      intros. 
+      eapply (@satisfiesAll_subst V Gamma Γf); eauto using agree_on_sym.
+      intros. inv H12.
+      intros.       
+      hnf in H30; dcr. 
+      eapply satisfiesAll_union; split; eauto.
+      eapply satisfiesAll_update_dead; eauto. rewrite map_length. 
+      exploit omap_length; eauto. congruence. 
+      simpl in *.
+      eapply (@satisfiesAll_subst V' Γ' Γf'); 
+        try eapply H7; eauto using agree_on_sym.
+      congruence. 
     - pfold. econstructor 3; try eapply star_refl. eauto. stuck; eauto.
       get_functional; subst. simpl in *. congruence.
     - pfold. econstructor 3; try eapply star_refl. eauto. stuck; eauto.
-  + simpl. hnf in H7; exploit H7; eauto. inv X; eauto.
+  + simpl. hnf in H8; exploit H8; eauto. inv X; eauto.
     - pfold. econstructor 3; try eapply star_refl. simpl. congruence.
       stuck.
     - pfold. econstructor 2; try eapply star_refl. simpl. congruence.
@@ -308,20 +654,45 @@ Proof.
     econstructor; eauto.
     econstructor; eauto.
     simpl. left. eapply IHs2; eauto.
-    - eapply H11; eauto.
-    - eapply H14; eauto.
+    - eapply H12; eauto.
+    - eapply H15; eauto.
     - eapply simL_mon; eauto. eapply simL_extension'; eauto.
       * hnf; intros. destruct a as [[[[Zb Γb] EqSb] Γb'] EqSb'].
-        hnf in H5. hnf in H6. dcr; subst.
+        hnf in H6. hnf in H7. dcr; subst.
         split; eauto. unfold var in *. congruence.
-      * hnf; intros. hnf in H5; dcr.
+      * hnf; intros. hnf in H6; dcr.
         eapply IHs1; eauto.
-        eapply H10. specialize (H23 V). eapply H23; eauto.
-        eapply H12. eapply H26; eauto.
-        destruct H10. rewrite H10. rewrite eqns_freeVars_union.
-         rewrite H18. rewrite H4. clear_all; cset_tac; intuition.
+        eapply H11. eauto. 
+        eapply H13. eauto.
+        eapply simL'_update; eauto.
+        unfold BlockRel. intros. 
+        destruct x as [[[[] ?] ?] ?]; dcr.
+        repeat (split; eauto).
+        symmetry. 
+        assert (eqns_freeVars s [=] eqns_freeVars s \ of_list Z) by admit.
+        rewrite H6.
+        eapply update_with_list_agree_minus. rewrite map_length; eauto.
+        eauto using agree_on_sym; eauto.
+        symmetry.
+        assert (eqns_freeVars s3 [=] eqns_freeVars s3 \ of_list Z) by admit.
+        rewrite H6.
+        eapply update_with_list_agree_minus. rewrite map_length; eauto.
+        eauto using agree_on_sym; eauto.
+        rewrite <- H35. clear_all; cset_tac; intuition. 
+        rewrite <- H37. clear_all; cset_tac; intuition.
+        destruct H11. rewrite H11. rewrite eqns_freeVars_union.
+        rewrite H19. rewrite H4. clear_all; cset_tac; intuition.
+        destruct H13. rewrite H13. rewrite eqns_freeVars_union.
+        rewrite H20. rewrite H5. clear_all; cset_tac; intuition.
       * hnf; split; eauto.
-    - destruct H11. rewrite H6; eauto.
+      * unfold entails in *. dcr. hnf; intros.
+        simpl. split.
+        rewrite <- H14. cset_tac; intuition. exfalso. eapply H14; eauto.
+        split.
+        rewrite <- H14. cset_tac; intuition. exfalso. eapply H14; eauto.
+        repeat (split; eauto using agree_on_refl).
+    - destruct H12. rewrite H7; eauto.
+    - destruct H15. rewrite H7; eauto.
 Qed.
 
 Print Assumptions sim_DVE.
